src/AM_St.v
@@ -1,4 +1,4 @@
-Require Import Maps BS Cvm_St ErrorStMonad_Coq.
+Require Import Maps BS Term_Defs_Core Cvm_St ErrorStMonad_Coq.
 
 
 Require Import List.
@@ -7,19 +7,24 @@ Import ListNotations.
 
 (* Specific AM monad state *)
 Record AM_St : Type := mkAM_St
-                         { am_nonceMap : MapC nat BS;
-                           am_nonceId : nat (* ;
+                         { am_nonceMap : MapC N_ID BS;
+                           am_nonceId : N_ID; 
+                           amConfig : AM_Config;
+                           
+                           (* ;
                            st_aspmap : asp_map;
                            st_sigmap : sig_map;
                            (*am_pl : Plc *)(*;
                            checked : list nat*) *) }.
 
 Definition empty_amst :=
-  mkAM_St map_empty 0 (* [] [] *) .
+  mkAM_St map_empty 0 empty_am_config (* [] [] *) .
+
 
 Inductive AM_Error : Type := 
 | cvm_error : CVM_Error -> AM_Error
-| am_error : StringT -> AM_Error.
+| am_error : StringT -> AM_Error
+| dispatch_error : DispatcherErrors -> AM_Error.
   (*
   | term_disclosure_error : Term -> AM_Error
   | manifest_asp_unavailable : ASP_ID ->   *)
