src/Appraisal_Defs.v
@@ -1,6 +1,6 @@
-Require Import Term_Defs_Core Term_Defs. (* OptMonad_Coq. *)
+Require Import Term_Defs_Core Term_Defs Manifest. (* OptMonad_Coq. *)
 
-Require Import Appraisal_IO_Stubs ErrorStMonad_Coq AM_Monad.
+Require Import Appraisal_IO_Stubs ErrorStMonad_Coq AM_Monad AM_St.
 
 (*
 Definition checkASP (params:ASP_PARAMS) (bs:BS) : Opt BS :=
@@ -20,8 +20,15 @@ Some (checkEE' params bs).
 Definition decrypt_bs_to_rawev' (bs:BS) (params:ASP_PARAMS) : AM RawEv :=
   ret (decrypt_bs_to_rawev bs params).
 
+Definition check_asp_EXTD (params:ASP_PARAMS) (p:Plc) (sig:BS) (ls:RawEv) (ac : AM_Config) : ResultT BS DispatcherErrors :=
+  ac.(app_aspCb) params p sig ls.
+
 Definition check_asp_EXTD' (params:ASP_PARAMS) (p:Plc) (sig:BS) (ls:RawEv) : AM BS :=
-  ret (check_asp_EXTD params p sig ls).
+  ac <- get_amConfig ;;
+  match (check_asp_EXTD params p sig ls ac) with
+  | resultC r => ret r
+  | errC e => failm (dispatch_error e)
+  end.
 
 Definition checkNonce' (nid:nat) (nonceCandidate:BS) : AM BS :=
   nonceGolden <- am_getNonce nid ;;
