src/ManCompSoundness_Appraisal.v
@@ -1,0 +1,240 @@
+Require Import Manifest Manifest_Compiler Manifest_Generator AbstractedTypes
+  Maps Term_Defs List Cvm_St Cvm_Impl ErrorStMonad_Coq StructTactics 
+  Cvm_Monad EqClass Manifest_Admits Auto.
+Require Import Manifest_Generator_Facts Executable_Defs_Prop 
+  Executable_Facts_Dist Eqb_Evidence.
+
+Require Import Coq.Program.Tactics.
+
+Import ListNotations.
+
+(* Set Nested Proofs Allowed. *)
+
+
+
+
+Definition supports_am_app (ac1 ac2 : AM_Config) : Prop :=
+  (forall aid l targ targid p' ev ev',
+      (forall res, 
+      ac1.(app_aspCb) (asp_paramsC aid l targ targid) p' ev ev' = resultC res ->
+      ac2.(app_aspCb) (asp_paramsC aid l targ targid) p' ev ev' = resultC res)) /\
+  (forall aid l targ targid p' ev ev',
+      ac1.(app_aspCb) (asp_paramsC aid l targ targid) p' ev ev' = errC Runtime ->
+      ac2.(app_aspCb) (asp_paramsC aid l targ targid) p' ev ev' = errC Runtime).
+
+Theorem supports_am_app_refl : forall ac1,
+  supports_am_app ac1 ac1.
+Proof.
+  unfold supports_am_app; intuition.
+Qed.
+
+Theorem supports_am_app_trans : forall ac1 ac2 ac3,
+  supports_am_app ac1 ac2 ->
+  supports_am_app ac2 ac3 ->
+  supports_am_app ac1 ac3.
+Proof.
+  unfold supports_am_app; intuition.
+Qed.
+
+Local Hint Resolve supports_am_app_refl : core.
+Local Hint Resolve supports_am_app_trans : core.
+
+Definition lib_supports_manifest_app (al : AM_Library) (am : Manifest) : Prop :=
+  (forall (a : (Plc*ASP_ID)), In a am.(appraisal_asps) -> exists cb, Maps.map_get al.(Local_Appraisal_ASPS) a = Some cb).
+
+(*
+Inductive Evidence: Set :=
+| mt: Evidence
+| nn: N_ID -> Evidence
+| uu: Plc -> FWD -> ASP_PARAMS -> Evidence -> Evidence
+| ss: Evidence -> Evidence -> Evidence.
+*)
+
+(*
+  | lseq t1 t2 =>
+      exists ac1 ac2,
+      (am_config_support_exec t1 p ac1) /\
+      (am_config_support_exec t2 p ac2) /\
+      supports_am ac1 ac /\
+      supports_am ac2 ac
+*)
+
+
+
+Fixpoint am_config_support_exec_app (e : Evidence) (ac : AM_Config) : Prop :=
+    match e with
+    | mt => True 
+    | nn _ => True (* TODO: how to account for nonce handling? *)
+    | uu p fwd ps e' => True 
+            (*
+            | ASPC _ _ (asp_paramsC aspid _ _ _) =>
+            (forall l targ targid p' ev ev',
+            ((exists res, 
+            ac.(aspCb) (asp_paramsC aspid l targ targid) p' ev ev' = resultC res) \/ 
+            ac.(aspCb) (asp_paramsC aspid l targ targid) p' ev ev' = errC Runtime))
+            *)
+    | ss e1 e2 => 
+        exists ac1 ac2, 
+        (am_config_support_exec_app e1 ac1) /\ 
+        (am_config_support_exec_app e1 ac1) /\ 
+        supports_am_app ac1 ac /\
+        supports_am_app ac2 ac
+    end.
+
+Require Import AM_St Impl_appraisal.
+
+Fixpoint nonce_ids_et (et:Evidence) : list N_ID.
+Admitted.
+
+Definition has_nonces (nids: list N_ID) (m:MapC N_ID BS) : Prop.
+Admitted.
+
+
+Theorem well_formed_am_config_impl_executable_app : forall et amConf ls,
+  am_config_support_exec_app et amConf ->
+  length ls = et_size et -> 
+  forall st,
+  supports_am_app amConf (st.(amConfig)) ->
+  has_nonces (nonce_ids_et et) (st.(am_nonceMap)) -> 
+    exists ec st',
+        (gen_appraise_AM et ls) st = (resultC ec, st') \/ 
+        (gen_appraise_AM et ls) st = (errC (dispatch_error Runtime), st'). 
+Proof.
+Admitted.
+
+Require Import ManCompSoundness.
+
+Definition manifest_support_am_config_app (m : Manifest) (ac : AM_Config) : Prop :=
+  (forall p a, In (p,a) (m.(appraisal_asps)) -> 
+    forall l targ targid ev ev',
+    (exists res, ac.(app_aspCb) (asp_paramsC a l targ targid) p ev ev' = resultC res) \/
+    (ac.(app_aspCb) (asp_paramsC a l targ targid) p ev ev' = errC Runtime)).
+
+Theorem manifest_support_am_config_compiler_app : forall absMan amLib,
+    lib_supports_manifest_app amLib absMan ->
+    manifest_support_am_config_app absMan (manifest_compiler absMan amLib).
+Proof.
+  unfold lib_supports_manifest_app, manifest_support_am_config_app, 
+    manifest_compiler, generate_PubKey_dispatcher, generate_Plc_dispatcher, generate_appraisal_ASP_dispatcher in *;
+  simpl in *; intuition;
+  repeat break_match; simpl in *; intuition; eauto;
+  match goal with
+  | H:  context[ map_get (minify_mapC ?l ?filt) ?a],
+    H1: forall a' : (Plc*ASP_ID), _ -> (exists x : _, map_get _ _ = Some x) |- _ => 
+    assert (CO : exists x, map_get (minify_mapC l filt) a = Some x)
+    ;
+      [
+      eapply filter_resolver; eauto;
+      repeat break_match; intuition; try congruence
+      | 
+      rewrite H in CO; destruct CO; congruence
+    ]
+  | H:  context[ map_get (minify_mapD ?l ?filt) ?a],
+    H1: forall a' : Plc, _ -> (exists x : _, map_get _ _ = Some x) |- _ => 
+    assert (CO : exists x, map_get (minify_mapD l filt) a = Some x)
+    ;
+      [
+      eapply filter_resolver_mapd; eauto;
+      repeat break_match; intuition; try congruence
+      | 
+      rewrite H in CO; destruct CO; congruence
+    ]
+  end.
+Qed.
+
+Fixpoint manifest_support_term_app (m : Manifest) (e : Evidence) : Prop :=
+    match e with
+    | mt => True 
+    | nn _ => True (* TODO: should we account for nonce presence here? *)
+    | uu p fwd ps e' => 
+        match ps with 
+        | asp_paramsC a _ _ _ => 
+            In (a,p) m.(appraisal_asps)
+        end
+        (* TODO:  support other fwd types here in the future... *)
+    | ss e1 e2 => 
+        manifest_support_term_app m e1 /\ 
+        manifest_support_term_app m e2
+    end.
+
+
+Theorem manifest_support_am_config_impl_am_config_app: forall et absMan amConf,
+    manifest_support_am_config_app absMan amConf ->
+    manifest_support_term_app absMan et ->
+    am_config_support_exec_app et amConf.
+Proof.
+    induction et; simpl in *; intuition; eauto;
+    unfold manifest_support_am_config_app in *; intuition; eauto;
+    repeat (try break_match; simpl in *; intuition; eauto).
+    - pose proof (IHet1 absMan amConf); 
+        pose proof (IHet2 absMan amConf); intuition;
+        exists amConf, amConf; eauto.
+Qed.
+
+Lemma manifest_supports_term_sub_app : forall m1 m2 et,
+manifest_subset m1 m2 ->
+manifest_support_term_app m1 et -> 
+manifest_support_term_app m2 et.
+Proof.
+  intros.
+  generalizeEverythingElse et.
+  induction et; intros; ff.
+  -
+    subst.
+    unfold manifest_subset in H. 
+    destruct_conjs.
+    ff.  
+  -
+    split; 
+    destruct_conjs; ff; eauto.
+Qed.
+
+Fixpoint manifest_generator_app' (et:Evidence) : Manifest. 
+Admitted.
+
+Theorem man_gen_old_always_supports_app : forall et absMan,
+  (* map_get (manifest_generator' tp t backMan) p = Some absMan -> *)
+  manifest_generator_app' et = absMan ->
+  manifest_support_term_app absMan et.
+Proof.
+Admitted.
+
+Theorem manifest_generator_compiler_soundness_app : forall et ls absMan amLib amConf,
+  (* map_get (manifest_generator t tp) p = Some absMan -> *)
+  manifest_generator_app' et = absMan ->
+  lib_supports_manifest_app amLib absMan ->
+  manifest_compiler absMan amLib = amConf ->
+  length ls = et_size et ->
+  forall st,
+
+  st.(amConfig) = amConf ->
+
+  has_nonces (nonce_ids_et et) (st.(am_nonceMap)) -> 
+
+    ( 
+
+    exists ec st',
+         (gen_appraise_AM et ls) st = (resultC ec, st') \/ 
+         (gen_appraise_AM et ls) st = (errC (dispatch_error Runtime), st')
+    ).
+Proof.
+  intros.
+  assert (supports_am_app amConf (st.(amConfig))) by ff.
+
+  eapply well_formed_am_config_impl_executable_app.
+  - unfold manifest_generator, e_empty in *; simpl in *.
+    eapply manifest_support_am_config_impl_am_config_app.
+    * eapply manifest_support_am_config_compiler_app; eauto.
+
+
+    * (* NOTE: This is the important one, substitute proof of any manifest here *)
+      eapply man_gen_old_always_supports_app; 
+      eassumption.
+
+  -
+  eassumption.
+  - 
+    rewrite H1; eauto.
+  - 
+   eassumption.
+Qed. 
